README.md
@@ -3,6 +3,7 @@
 Proofs:
 
 - Players alternate after each move
+- A cell get marked after each move
 
 Pending:
 
@@ -12,7 +13,7 @@ Pending:
 
 Other interesting proofs we could write:
 
--- The game ends after a maximum of 9 valid moves
+-- The game ends after a maximum of 9 moves
 -- If the board has a winning line after X moves, the game is in the Win state.
 -- If the board has a winning line after X moves, there are no other winning lines.
 -- If there is a draw, there are no winning lines.
